more symbols;

thys/Functional-Automata/AutoMaxChop.thy
@@ -8,22 +8,22 @@ theory AutoMaxChop
 imports DA MaxChop
 begin
 
-primrec auto_split :: "('a,'s)da => 's  => 'a list * 'a list => 'a list => 'a splitter" where
+primrec auto_split :: "('a,'s)da \<Rightarrow> 's  \<Rightarrow> 'a list * 'a list \<Rightarrow> 'a list \<Rightarrow> 'a splitter" where
 "auto_split A q res ps []     = (if fin A q then (ps,[]) else res)" |
 "auto_split A q res ps (x#xs) =
    auto_split A (next A x q) (if fin A q then (ps,x#xs) else res) (ps@[x]) xs"
 
 definition
- auto_chop :: "('a,'s)da => 'a chopper" where
-"auto_chop A = chop (%xs. auto_split A (start A) ([],xs) [] xs)"
+ auto_chop :: "('a,'s)da \<Rightarrow> 'a chopper" where
+"auto_chop A = chop (\<lambda>xs. auto_split A (start A) ([],xs) [] xs)"
 
 
 lemma delta_snoc: "delta A (xs@[y]) q = next A y (delta A xs q)"
 by simp
 
 lemma auto_split_lemma:
- "!!q ps res. auto_split A (delta A ps q) res ps xs =
-              maxsplit (%ys. fin A (delta A ys q)) res ps xs"
+ "\<And>q ps res. auto_split A (delta A ps q) res ps xs =
+              maxsplit (\<lambda>ys. fin A (delta A ys q)) res ps xs"
 apply (induct xs)
  apply simp
 apply (simp add: delta_snoc[symmetric] del: delta_append)
@@ -38,7 +38,7 @@ apply simp
 done
 
 lemma is_maxsplitter_auto_split:
- "is_maxsplitter (accepts A) (%xs. auto_split A (start A) ([],xs) [] xs)"
+ "is_maxsplitter (accepts A) (\<lambda>xs. auto_split A (start A) ([],xs) [] xs)"
 by (simp add: auto_split_is_maxsplit is_maxsplitter_maxsplit)
 
 
