thys/Functional-Automata/MaxPrefix.thy
@@ -9,18 +9,18 @@ imports "HOL-Library.Sublist"
 begin
 
 definition
- is_maxpref :: "('a list => bool) => 'a list => 'a list => bool" where
+ is_maxpref :: "('a list \<Rightarrow> bool) \<Rightarrow> 'a list \<Rightarrow> 'a list \<Rightarrow> bool" where
 "is_maxpref P xs ys =
- (prefix xs ys & (xs=[] | P xs) & (!zs. prefix zs ys & P zs --> prefix zs xs))"
+ (prefix xs ys \<and> (xs=[] \<or> P xs) \<and> (\<forall>zs. prefix zs ys \<and> P zs \<longrightarrow> prefix zs xs))"
 
-type_synonym 'a splitter = "'a list => 'a list * 'a list"
+type_synonym 'a splitter = "'a list \<Rightarrow> 'a list * 'a list"
 
 definition
- is_maxsplitter :: "('a list => bool) => 'a splitter => bool" where
+ is_maxsplitter :: "('a list \<Rightarrow> bool) \<Rightarrow> 'a splitter \<Rightarrow> bool" where
 "is_maxsplitter P f =
- (!xs ps qs. f xs = (ps,qs) = (xs=ps@qs & is_maxpref P ps xs))"
+ (\<forall>xs ps qs. f xs = (ps,qs) = (xs=ps@qs \<and> is_maxpref P ps xs))"
 
-fun maxsplit :: "('a list => bool) => 'a list * 'a list => 'a list => 'a splitter" where
+fun maxsplit :: "('a list \<Rightarrow> bool) \<Rightarrow> 'a list * 'a list \<Rightarrow> 'a list \<Rightarrow> 'a splitter" where
 "maxsplit P res ps []     = (if P ps then (ps,[]) else res)" |
 "maxsplit P res ps (q#qs) = maxsplit P (if P ps then (ps,q#qs) else res)
                                      (ps@[q]) qs"
@@ -36,18 +36,18 @@ proof (induction P res ps qs rule: maxsplit.induct)
 next
   case (2 P res ps q qs)
   show ?case
-  proof (cases "\<exists>us. prefix us qs & P ((ps @ [q]) @ us)")
+  proof (cases "\<exists>us. prefix us qs \<and> P ((ps @ [q]) @ us)")
     case True
     note ex1 = this
     then guess us by (elim exE conjE) note us = this
-    hence ex2: "\<exists>us. prefix us (q # qs) & P (ps @ us)"
+    hence ex2: "\<exists>us. prefix us (q # qs) \<and> P (ps @ us)"
       by (intro exI[of _ "q#us"]) auto
     with ex1 and 2 show ?thesis by simp
   next
     case False
     note ex1 = this
     show ?thesis
-    proof (cases "\<exists>us. prefix us (q#qs) & P (ps @ us)")
+    proof (cases "\<exists>us. prefix us (q#qs) \<and> P (ps @ us)")
       case False
       from 2 show ?thesis
         by (simp only: ex1 False) (insert ex1 False, auto simp: prefix_Cons)
@@ -84,7 +84,7 @@ lemma is_maxpref_Nil[simp]:
   by (auto simp: is_maxpref_def)
 
 lemma is_maxsplitter_maxsplit:
- "is_maxsplitter P (%xs. maxsplit P ([],xs) [] xs)"
+ "is_maxsplitter P (\<lambda>xs. maxsplit P ([],xs) [] xs)"
   by (auto simp: maxsplit_lemma is_maxsplitter_def)
 
 lemmas maxsplit_eq = is_maxsplitter_maxsplit[simplified is_maxsplitter_def]
