thys/Functional-Automata/NA.thy
@@ -8,21 +8,21 @@ theory NA
 imports AutoProj
 begin
 
-type_synonym ('a,'s) na = "'s * ('a => 's => 's set) * ('s => bool)"
+type_synonym ('a,'s) na = "'s * ('a \<Rightarrow> 's \<Rightarrow> 's set) * ('s \<Rightarrow> bool)"
 
-primrec delta :: "('a,'s)na => 'a list => 's => 's set" where
+primrec delta :: "('a,'s)na \<Rightarrow> 'a list \<Rightarrow> 's \<Rightarrow> 's set" where
 "delta A []    p = {p}" |
 "delta A (a#w) p = Union(delta A w ` next A a p)"
 
 definition
- accepts :: "('a,'s)na => 'a list => bool" where
-"accepts A w = (EX q : delta A w (start A). fin A q)"
+ accepts :: "('a,'s)na \<Rightarrow> 'a list \<Rightarrow> bool" where
+"accepts A w = (\<exists>q \<in> delta A w (start A). fin A q)"
 
 definition
- step :: "('a,'s)na => 'a => ('s * 's)set" where
+ step :: "('a,'s)na \<Rightarrow> 'a \<Rightarrow> ('s * 's)set" where
 "step A a = {(p,q) . q : next A a p}"
 
-primrec steps :: "('a,'s)na => 'a list => ('s * 's)set" where
+primrec steps :: "('a,'s)na \<Rightarrow> 'a list \<Rightarrow> ('s * 's)set" where
 "steps A [] = Id" |
 "steps A (a#w) = step A a  O  steps A w"
 
@@ -36,15 +36,15 @@ apply(rule steps_append[THEN equalityE])
 apply blast
 done
 
-lemma delta_conv_steps: "!!p. delta A w p = {q. (p,q) : steps A w}"
+lemma delta_conv_steps: "\<And>p. delta A w p = {q. (p,q) : steps A w}"
 by(induct w)(auto simp:step_def)
 
 lemma accepts_conv_steps:
- "accepts A w = (? q. (start A,q) : steps A w & fin A q)"
+ "accepts A w = (\<exists>q. (start A,q) \<in> steps A w \<and> fin A q)"
 by(simp add: delta_conv_steps accepts_def)
 
 abbreviation
-  Cons_syn :: "'a => 'a list set => 'a list set" (infixr "##" 65) where
-  "x ## S == Cons x ` S"
+  Cons_syn :: "'a \<Rightarrow> 'a list set \<Rightarrow> 'a list set" (infixr "##" 65) where
+  "x ## S \<equiv> Cons x ` S"
 
 end
