thys/Functional-Automata/RegExp2NAe.thy
@@ -12,48 +12,48 @@ type_synonym 'a bitsNAe = "('a,bool list)nae"
 
 definition
  epsilon :: "'a bitsNAe" where
-"epsilon = ([],%a s. {}, %s. s=[])"
+"epsilon = ([],\<lambda>a s. {}, \<lambda>s. s=[])"
 
 definition
-"atom"  :: "'a => 'a bitsNAe" where
+"atom"  :: "'a \<Rightarrow> 'a bitsNAe" where
 "atom a = ([True],
-            %b s. if s=[True] & b=Some a then {[False]} else {},
-            %s. s=[False])"
+            \<lambda>b s. if s=[True] \<and> b=Some a then {[False]} else {},
+            \<lambda>s. s=[False])"
 
 definition
- or :: "'a bitsNAe => 'a bitsNAe => 'a bitsNAe" where
-"or = (%(ql,dl,fl)(qr,dr,fr).
+ or :: "'a bitsNAe \<Rightarrow> 'a bitsNAe \<Rightarrow> 'a bitsNAe" where
+"or = (\<lambda>(ql,dl,fl)(qr,dr,fr).
    ([],
-    %a s. case s of
-            [] => if a=None then {True#ql,False#qr} else {}
-          | left#s => if left then True ## dl a s
+    \<lambda>a s. case s of
+            [] \<Rightarrow> if a=None then {True#ql,False#qr} else {}
+          | left#s \<Rightarrow> if left then True ## dl a s
                               else False ## dr a s,
-    %s. case s of [] => False | left#s => if left then fl s else fr s))"
+    \<lambda>s. case s of [] \<Rightarrow> False | left#s \<Rightarrow> if left then fl s else fr s))"
 
 definition
- conc :: "'a bitsNAe => 'a bitsNAe => 'a bitsNAe" where
-"conc = (%(ql,dl,fl)(qr,dr,fr).
+ conc :: "'a bitsNAe \<Rightarrow> 'a bitsNAe \<Rightarrow> 'a bitsNAe" where
+"conc = (\<lambda>(ql,dl,fl)(qr,dr,fr).
    (True#ql,
-    %a s. case s of
-            [] => {}
-          | left#s => if left then (True ## dl a s) Un
-                                   (if fl s & a=None then {False#qr} else {})
+    \<lambda>a s. case s of
+            [] \<Rightarrow> {}
+          | left#s \<Rightarrow> if left then (True ## dl a s) \<union>
+                                   (if fl s \<and> a=None then {False#qr} else {})
                               else False ## dr a s,
-    %s. case s of [] => False | left#s => ~left & fr s))"
+    \<lambda>s. case s of [] \<Rightarrow> False | left#s \<Rightarrow> \<not>left \<and> fr s))"
 
 definition
- star :: "'a bitsNAe => 'a bitsNAe" where
-"star = (%(q,d,f).
+ star :: "'a bitsNAe \<Rightarrow> 'a bitsNAe" where
+"star = (\<lambda>(q,d,f).
    ([],
-    %a s. case s of
-            [] => if a=None then {True#q} else {}
-          | left#s => if left then (True ## d a s) Un
-                                   (if f s & a=None then {True#q} else {})
+    \<lambda>a s. case s of
+            [] \<Rightarrow> if a=None then {True#q} else {}
+          | left#s \<Rightarrow> if left then (True ## d a s) \<union>
+                                   (if f s \<and> a=None then {True#q} else {})
                               else {},
-    %s. case s of [] => True | left#s => left & f s))"
+    \<lambda>s. case s of [] \<Rightarrow> True | left#s \<Rightarrow> left \<and> f s))"
 
-primrec rexp2nae :: "'a rexp => 'a bitsNAe" where
-"rexp2nae Zero       = ([], %a s. {}, %s. False)" |
+primrec rexp2nae :: "'a rexp \<Rightarrow> 'a bitsNAe" where
+"rexp2nae Zero       = ([], \<lambda>a s. {}, \<lambda>s. False)" |
 "rexp2nae One        = epsilon" |
 "rexp2nae(Atom a)    = atom a" |
 "rexp2nae(Plus r s)  = or   (rexp2nae r) (rexp2nae s)" |
@@ -69,7 +69,7 @@ declare split_paired_all[simp]
 lemma step_epsilon[simp]: "step epsilon a = {}"
 by(simp add:epsilon_def step_def)
 
-lemma steps_epsilon: "((p,q) : steps epsilon w) = (w=[] & p=q)"
+lemma steps_epsilon: "((p,q) : steps epsilon w) = (w=[] \<and> p=q)"
 by (induct "w") auto
 
 lemma accepts_epsilon[simp]: "accepts epsilon w = (w = [])"
@@ -94,7 +94,7 @@ lemma eps_atom[simp]:
 by (simp add:atom_def step_def)
 
 lemma in_step_atom_Some[simp]:
- "(p,q) : step (atom a) (Some b) = (p=[True] & q=[False] & b=a)"
+ "(p,q) : step (atom a) (Some b) = (p=[True] \<and> q=[False] \<and> b=a)"
 by (simp add:atom_def step_def)
 
 lemma False_False_in_steps_atom:
@@ -122,23 +122,23 @@ by (simp add: accepts_def start_fin_in_steps_atom fin_atom)
 (***** lift True/False over fin *****)
 
 lemma fin_or_True[iff]:
- "!!L R. fin (or L R) (True#p) = fin L p"
+ "\<And>L R. fin (or L R) (True#p) = fin L p"
 by(simp add:or_def)
 
 lemma fin_or_False[iff]:
- "!!L R. fin (or L R) (False#p) = fin R p"
+ "\<And>L R. fin (or L R) (False#p) = fin R p"
 by(simp add:or_def)
 
 (***** lift True/False over step *****)
 
 lemma True_in_step_or[iff]:
-"!!L R. (True#p,q) : step (or L R) a = (? r. q = True#r & (p,r) : step L a)"
+"\<And>L R. (True#p,q) : step (or L R) a = (\<exists>r. q = True#r \<and> (p,r) : step L a)"
 apply (simp add:or_def step_def)
 apply blast
 done
 
 lemma False_in_step_or[iff]:
-"!!L R. (False#p,q) : step (or L R) a = (? r. q = False#r & (p,r) : step R a)"
+"\<And>L R. (False#p,q) : step (or L R) a = (\<exists>r. q = False#r \<and> (p,r) : step R a)"
 apply (simp add:or_def step_def)
 apply blast
 done
@@ -147,8 +147,8 @@ done
 (***** lift True/False over epsclosure *****)
 
 lemma lemma1a:
- "(tp,tq) : (eps(or L R))^* ==> 
- (!!p. tp = True#p ==> ? q. (p,q) : (eps L)^* & tq = True#q)"
+ "(tp,tq) : (eps(or L R))\<^sup>* \<Longrightarrow> 
+ (\<And>p. tp = True#p \<Longrightarrow> \<exists>q. (p,q) : (eps L)\<^sup>* \<and> tq = True#q)"
 apply (induct rule:rtrancl_induct)
  apply (blast)
 apply (clarify)
@@ -157,8 +157,8 @@ apply (blast intro: rtrancl_into_rtrancl)
 done
 
 lemma lemma1b:
- "(tp,tq) : (eps(or L R))^* ==> 
- (!!p. tp = False#p ==> ? q. (p,q) : (eps R)^* & tq = False#q)"
+ "(tp,tq) : (eps(or L R))\<^sup>* \<Longrightarrow> 
+ (\<And>p. tp = False#p \<Longrightarrow> \<exists>q. (p,q) : (eps R)\<^sup>* \<and> tq = False#q)"
 apply (induct rule:rtrancl_induct)
  apply (blast)
 apply (clarify)
@@ -167,38 +167,38 @@ apply (blast intro: rtrancl_into_rtrancl)
 done
 
 lemma lemma2a:
- "(p,q) : (eps L)^*  ==> (True#p, True#q) : (eps(or L R))^*"
+ "(p,q) : (eps L)\<^sup>*  \<Longrightarrow> (True#p, True#q) : (eps(or L R))\<^sup>*"
 apply (induct rule: rtrancl_induct)
  apply (blast)
 apply (blast intro: rtrancl_into_rtrancl)
 done
 
 lemma lemma2b:
- "(p,q) : (eps R)^*  ==> (False#p, False#q) : (eps(or L R))^*"
+ "(p,q) : (eps R)\<^sup>*  \<Longrightarrow> (False#p, False#q) : (eps(or L R))\<^sup>*"
 apply (induct rule: rtrancl_induct)
  apply (blast)
 apply (blast intro: rtrancl_into_rtrancl)
 done
 
 lemma True_epsclosure_or[iff]:
- "(True#p,q) : (eps(or L R))^* = (? r. q = True#r & (p,r) : (eps L)^*)"
+ "(True#p,q) : (eps(or L R))\<^sup>* = (\<exists>r. q = True#r \<and> (p,r) : (eps L)\<^sup>*)"
 by (blast dest: lemma1a lemma2a)
 
 lemma False_epsclosure_or[iff]:
- "(False#p,q) : (eps(or L R))^* = (? r. q = False#r & (p,r) : (eps R)^*)"
+ "(False#p,q) : (eps(or L R))\<^sup>* = (\<exists>r. q = False#r \<and> (p,r) : (eps R)\<^sup>*)"
 by (blast dest: lemma1b lemma2b)
 
 (***** lift True/False over steps *****)
 
 lemma lift_True_over_steps_or[iff]:
- "!!p. (True#p,q):steps (or L R) w = (? r. q = True # r & (p,r):steps L w)"
+ "\<And>p. (True#p,q):steps (or L R) w = (\<exists>r. q = True # r \<and> (p,r):steps L w)"
 apply (induct "w")
  apply auto
 apply force
 done
 
 lemma lift_False_over_steps_or[iff]:
- "!!p. (False#p,q):steps (or L R) w = (? r. q = False#r & (p,r):steps R w)"
+ "\<And>p. (False#p,q):steps (or L R) w = (\<exists>r. q = False#r \<and> (p,r):steps R w)"
 apply (induct "w")
  apply auto
 apply (force)
@@ -207,7 +207,7 @@ done
 (***** Epsilon closure of start state *****)
 
 lemma unfold_rtrancl2:
- "R^* = Id Un (R O R^*)"
+ "R\<^sup>* = Id \<union> (R O R\<^sup>*)"
 apply (rule set_eqI)
 apply (simp)
 apply (rule iffI)
@@ -218,7 +218,7 @@ apply (blast intro: converse_rtrancl_into_rtrancl)
 done
 
 lemma in_unfold_rtrancl2:
- "(p,q) : R^* = (q = p | (? r. (p,r) : R & (r,q) : R^*))"
+ "(p,q) : R\<^sup>* = (q = p | (\<exists>r. (p,r) : R \<and> (r,q) : R\<^sup>*))"
 apply (rule unfold_rtrancl2[THEN equalityE])
 apply (blast)
 done
@@ -226,19 +226,19 @@ done
 lemmas [iff] = in_unfold_rtrancl2[where ?p = "start(or L R)"] for L R
 
 lemma start_eps_or[iff]:
- "!!L R. (start(or L R),q) : eps(or L R) = 
+ "\<And>L R. (start(or L R),q) : eps(or L R) = 
        (q = True#start L | q = False#start R)"
 by (simp add:or_def step_def)
 
 lemma not_start_step_or_Some[iff]:
- "!!L R. (start(or L R),q) ~: step (or L R) (Some a)"
+ "\<And>L R. (start(or L R),q) \<notin> step (or L R) (Some a)"
 by (simp add:or_def step_def)
 
 lemma steps_or:
  "(start(or L R), q) : steps (or L R) w = 
- ( (w = [] & q = start(or L R)) | 
-   (? p.  q = True  # p & (start L,p) : steps L w | 
-          q = False # p & (start R,p) : steps R w) )"
+ ( (w = [] \<and> q = start(or L R)) | 
+   (\<exists>p.  q = True  # p \<and> (start L,p) : steps L w | 
+         q = False # p \<and> (start R,p) : steps R w) )"
 apply (case_tac "w")
  apply (simp)
  apply (blast)
@@ -247,7 +247,7 @@ apply (blast)
 done
 
 lemma start_or_not_final[iff]:
- "!!L R. ~ fin (or L R) (start(or L R))"
+ "\<And>L R. \<not> fin (or L R) (start(or L R))"
 by (simp add:or_def)
 
 lemma accepts_or:
@@ -264,46 +264,46 @@ done
 (** True/False in fin **)
 
 lemma in_conc_True[iff]:
- "!!L R. fin (conc L R) (True#p) = False"
+ "\<And>L R. fin (conc L R) (True#p) = False"
 by (simp add:conc_def)
 
 lemma fin_conc_False[iff]:
- "!!L R. fin (conc L R) (False#p) = fin R p"
+ "\<And>L R. fin (conc L R) (False#p) = fin R p"
 by (simp add:conc_def)
 
 (** True/False in step **)
 
 lemma True_step_conc[iff]:
- "!!L R. (True#p,q) : step (conc L R) a = 
-       ((? r. q=True#r & (p,r): step L a) | 
-        (fin L p & a=None & q=False#start R))"
+ "\<And>L R. (True#p,q) : step (conc L R) a = 
+       ((\<exists>r. q=True#r \<and> (p,r): step L a) | 
+        (fin L p \<and> a=None \<and> q=False#start R))"
 by (simp add:conc_def step_def) (blast)
 
 lemma False_step_conc[iff]:
- "!!L R. (False#p,q) : step (conc L R) a = 
-       (? r. q = False#r & (p,r) : step R a)"
+ "\<And>L R. (False#p,q) : step (conc L R) a = 
+       (\<exists>r. q = False#r \<and> (p,r) : step R a)"
 by (simp add:conc_def step_def) (blast)
 
 (** False in epsclosure **)
 
 lemma lemma1b':
- "(tp,tq) : (eps(conc L R))^* ==> 
-  (!!p. tp = False#p ==> ? q. (p,q) : (eps R)^* & tq = False#q)"
+ "(tp,tq) : (eps(conc L R))\<^sup>* \<Longrightarrow> 
+  (\<And>p. tp = False#p \<Longrightarrow> \<exists>q. (p,q) : (eps R)\<^sup>* \<and> tq = False#q)"
 apply (induct rule: rtrancl_induct)
  apply (blast)
 apply (blast intro: rtrancl_into_rtrancl)
 done
 
 lemma lemma2b':
- "(p,q) : (eps R)^* ==> (False#p, False#q) : (eps(conc L R))^*"
+ "(p,q) : (eps R)\<^sup>* \<Longrightarrow> (False#p, False#q) : (eps(conc L R))\<^sup>*"
 apply (induct rule: rtrancl_induct)
  apply (blast)
 apply (blast intro: rtrancl_into_rtrancl)
 done
 
 lemma False_epsclosure_conc[iff]:
- "((False # p, q) : (eps (conc L R))^*) = 
- (? r. q = False # r & (p, r) : (eps R)^*)"
+ "((False # p, q) : (eps (conc L R))\<^sup>*) = 
+ (\<exists>r. q = False # r \<and> (p, r) : (eps R)\<^sup>*)"
 apply (rule iffI)
  apply (blast dest: lemma1b')
 apply (blast dest: lemma2b')
@@ -312,7 +312,7 @@ done
 (** False in steps **)
 
 lemma False_steps_conc[iff]:
- "!!p. (False#p,q): steps (conc L R) w = (? r. q=False#r & (p,r): steps R w)"
+ "\<And>p. (False#p,q): steps (conc L R) w = (\<exists>r. q=False#r \<and> (p,r): steps R w)"
 apply (induct "w")
  apply (simp)
 apply (simp)
@@ -322,14 +322,14 @@ done
 (** True in epsclosure **)
 
 lemma True_True_eps_concI:
- "(p,q): (eps L)^* ==> (True#p,True#q) : (eps(conc L R))^*"
+ "(p,q): (eps L)\<^sup>* \<Longrightarrow> (True#p,True#q) : (eps(conc L R))\<^sup>*"
 apply (induct rule: rtrancl_induct)
  apply (blast)
 apply (blast intro: rtrancl_into_rtrancl)
 done
 
 lemma True_True_steps_concI:
- "!!p. (p,q) : steps L w ==> (True#p,True#q) : steps (conc L R) w"
+ "\<And>p. (p,q) : steps L w \<Longrightarrow> (True#p,True#q) : steps (conc L R) w"
 apply (induct "w")
  apply (simp add: True_True_eps_concI)
 apply (simp)
@@ -337,28 +337,28 @@ apply (blast intro: True_True_eps_concI)
 done
 
 lemma lemma1a':
- "(tp,tq) : (eps(conc L R))^* ==> 
- (!!p. tp = True#p ==> 
-  (? q. tq = True#q & (p,q) : (eps L)^*) | 
-  (? q r. tq = False#q & (p,r):(eps L)^* & fin L r & (start R,q) : (eps R)^*))"
+ "(tp,tq) : (eps(conc L R))\<^sup>* \<Longrightarrow> 
+ (\<And>p. tp = True#p \<Longrightarrow> 
+  (\<exists>q. tq = True#q \<and> (p,q) : (eps L)\<^sup>*) | 
+  (\<exists>q r. tq = False#q \<and> (p,r):(eps L)\<^sup>* \<and> fin L r \<and> (start R,q) : (eps R)\<^sup>*))"
 apply (induct rule: rtrancl_induct)
  apply (blast)
 apply (blast intro: rtrancl_into_rtrancl)
 done
 
 lemma lemma2a':
- "(p, q) : (eps L)^* ==> (True#p, True#q) : (eps(conc L R))^*"
+ "(p, q) : (eps L)\<^sup>* \<Longrightarrow> (True#p, True#q) : (eps(conc L R))\<^sup>*"
 apply (induct rule: rtrancl_induct)
  apply (blast)
 apply (blast intro: rtrancl_into_rtrancl)
 done
 
 lemma lem:
- "!!L R. (p,q) : step R None ==> (False#p, False#q) : step (conc L R) None"
+ "\<And>L R. (p,q) : step R None \<Longrightarrow> (False#p, False#q) : step (conc L R) None"
 by(simp add: conc_def step_def)
 
 lemma lemma2b'':
- "(p,q) : (eps R)^* ==> (False#p, False#q) : (eps(conc L R))^*"
+ "(p,q) : (eps R)\<^sup>* \<Longrightarrow> (False#p, False#q) : (eps(conc L R))\<^sup>*"
 apply (induct rule: rtrancl_induct)
  apply (blast)
 apply (drule lem)
@@ -366,14 +366,14 @@ apply (blast intro: rtrancl_into_rtrancl)
 done
 
 lemma True_False_eps_concI:
- "!!L R. fin L p ==> (True#p, False#start R) : eps(conc L R)"
+ "\<And>L R. fin L p \<Longrightarrow> (True#p, False#start R) : eps(conc L R)"
 by(simp add: conc_def step_def)
 
 lemma True_epsclosure_conc[iff]:
- "((True#p,q) : (eps(conc L R))^*) = 
- ((? r. (p,r) : (eps L)^* & q = True#r) | 
-  (? r. (p,r) : (eps L)^* & fin L r & 
-        (? s. (start R, s) : (eps R)^* & q = False#s)))"
+ "((True#p,q) \<in> (eps(conc L R))\<^sup>*) = 
+ ((\<exists>r. (p,r) \<in> (eps L)\<^sup>* \<and> q = True#r) \<or>
+  (\<exists>r. (p,r) \<in> (eps L)\<^sup>* \<and> fin L r \<and>
+        (\<exists>s. (start R, s) \<in> (eps R)\<^sup>* \<and> q = False#s)))"
 apply (rule iffI)
  apply (blast dest: lemma1a')
 apply (erule disjE)
@@ -389,10 +389,10 @@ done
 (** True in steps **)
 
 lemma True_steps_concD[rule_format]:
- "!p. (True#p,q) : steps (conc L R) w --> 
-     ((? r. (p,r) : steps L w & q = True#r)  | 
-      (? u v. w = u@v & (? r. (p,r) : steps L u & fin L r & 
-              (? s. (start R,s) : steps R v & q = False#s))))"
+ "\<forall>p. (True#p,q) : steps (conc L R) w \<longrightarrow> 
+     ((\<exists>r. (p,r) : steps L w \<and> q = True#r)  \<or>
+      (\<exists>u v. w = u@v \<and> (\<exists>r. (p,r) \<in> steps L u \<and> fin L r \<and>
+              (\<exists>s. (start R,s) \<in> steps R v \<and> q = False#s))))"
 apply (induct "w")
  apply (simp)
 apply (simp)
@@ -420,25 +420,25 @@ apply (blast)
 done
 
 lemma True_steps_conc:
- "(True#p,q) : steps (conc L R) w = 
- ((? r. (p,r) : steps L w & q = True#r)  | 
-  (? u v. w = u@v & (? r. (p,r) : steps L u & fin L r & 
-          (? s. (start R,s) : steps R v & q = False#s))))"
+ "(True#p,q) \<in> steps (conc L R) w = 
+ ((\<exists>r. (p,r) \<in> steps L w \<and> q = True#r)  | 
+  (\<exists>u v. w = u@v \<and> (\<exists>r. (p,r) : steps L u \<and> fin L r \<and> 
+          (\<exists>s. (start R,s) : steps R v \<and> q = False#s))))"
 by (blast dest: True_steps_concD
     intro: True_True_steps_concI in_steps_epsclosure)
 
 (** starting from the start **)
 
 lemma start_conc:
-  "!!L R. start(conc L R) = True#start L"
+  "\<And>L R. start(conc L R) = True#start L"
 by (simp add: conc_def)
 
 lemma final_conc:
- "!!L R. fin(conc L R) p = (? s. p = False#s & fin R s)"
+ "\<And>L R. fin(conc L R) p = (\<exists>s. p = False#s \<and> fin R s)"
 by (simp add:conc_def split: list.split)
 
 lemma accepts_conc:
- "accepts (conc L R) w = (? u v. w = u@v & accepts L u & accepts R v)"
+ "accepts (conc L R) w = (\<exists>u v. w = u@v \<and> accepts L u \<and> accepts R v)"
 apply (simp add: accepts_def True_steps_conc final_conc start_conc)
 apply (blast)
 done
@@ -448,29 +448,29 @@ done
 (******************************************************)
 
 lemma True_in_eps_star[iff]:
- "!!A. (True#p,q) : eps(star A) = 
-     ( (? r. q = True#r & (p,r) : eps A) | (fin A p & q = True#start A) )"
+ "\<And>A. (True#p,q) \<in> eps(star A) = 
+     ( (\<exists>r. q = True#r \<and> (p,r) \<in> eps A) \<or> (fin A p \<and> q = True#start A) )"
 by (simp add:star_def step_def) (blast)
 
 lemma True_True_step_starI:
-  "!!A. (p,q) : step A a ==> (True#p, True#q) : step (star A) a"
+  "\<And>A. (p,q) : step A a \<Longrightarrow> (True#p, True#q) : step (star A) a"
 by (simp add:star_def step_def)
 
 lemma True_True_eps_starI:
-  "(p,r) : (eps A)^* ==> (True#p, True#r) : (eps(star A))^*"
+  "(p,r) : (eps A)\<^sup>* \<Longrightarrow> (True#p, True#r) : (eps(star A))\<^sup>*"
 apply (induct rule: rtrancl_induct)
  apply (blast)
 apply (blast intro: True_True_step_starI rtrancl_into_rtrancl)
 done
 
 lemma True_start_eps_starI:
- "!!A. fin A p ==> (True#p,True#start A) : eps(star A)"
+ "\<And>A. fin A p \<Longrightarrow> (True#p,True#start A) : eps(star A)"
 by (simp add:star_def step_def)
 
 lemma lem':
- "(tp,s) : (eps(star A))^* ==> (! p. tp = True#p --> 
- (? r. ((p,r) : (eps A)^* | 
-        (? q. (p,q) : (eps A)^* & fin A q & (start A,r) : (eps A)^*)) & 
+ "(tp,s) : (eps(star A))\<^sup>* \<Longrightarrow> (\<forall>p. tp = True#p \<longrightarrow>
+ (\<exists>r. ((p,r) \<in> (eps A)\<^sup>* \<or>
+        (\<exists>q. (p,q) \<in> (eps A)\<^sup>* \<and> fin A q \<and> (start A,r) : (eps A)\<^sup>*)) \<and> 
        s = True#r))"
 apply (induct rule: rtrancl_induct)
  apply (simp)
@@ -480,9 +480,9 @@ apply (blast intro: rtrancl_into_rtrancl)
 done
 
 lemma True_eps_star[iff]:
- "((True#p,s) : (eps(star A))^*) = 
- (? r. ((p,r) : (eps A)^* | 
-        (? q. (p,q) : (eps A)^* & fin A q & (start A,r) : (eps A)^*)) & 
+ "((True#p,s) \<in> (eps(star A))\<^sup>*) = 
+ (\<exists>r. ((p,r) \<in> (eps A)\<^sup>* \<or>
+        (\<exists>q. (p,q) : (eps A)\<^sup>* \<and> fin A q \<and> (start A,r) : (eps A)\<^sup>*)) \<and>
        s = True#r)"
 apply (rule iffI)
  apply (drule lem')
@@ -503,8 +503,8 @@ done
 (** True in step Some **)
 
 lemma True_step_star[iff]:
- "!!A. (True#p,r): step (star A) (Some a) = 
-     (? q. (p,q): step A (Some a) & r=True#q)"
+ "\<And>A. (True#p,r) \<in> step (star A) (Some a) =
+     (\<exists>q. (p,q) \<in> step A (Some a) \<and> r=True#q)"
 by (simp add:star_def step_def) (blast)
 
 
@@ -512,10 +512,10 @@ by (simp add:star_def step_def) (blast)
 
 (* reverse list induction! Complicates matters for conc? *)
 lemma True_start_steps_starD[rule_format]:
- "!rr. (True#start A,rr) : steps (star A) w --> 
- (? us v. w = concat us @ v & 
-             (!u:set us. accepts A u) & 
-             (? r. (start A,r) : steps A v & rr = True#r))"
+ "\<forall>rr. (True#start A,rr) \<in> steps (star A) w \<longrightarrow>
+ (\<exists>us v. w = concat us @ v \<and>
+             (\<forall>u\<in>set us. accepts A u) \<and>
+             (\<exists>r. (start A,r) \<in> steps A v \<and> rr = True#r))"
 apply (induct w rule: rev_induct)
  apply (simp)
  apply (clarify)
@@ -541,7 +541,7 @@ apply (blast)
 done
 
 lemma True_True_steps_starI:
-  "!!p. (p,q) : steps A w ==> (True#p,True#q) : steps (star A) w"
+  "\<And>p. (p,q) : steps A w \<Longrightarrow> (True#p,True#q) : steps (star A) w"
 apply (induct "w")
  apply (simp)
 apply (simp)
@@ -549,8 +549,8 @@ apply (blast intro: True_True_eps_starI True_True_step_starI)
 done
 
 lemma steps_star_cycle:
- "(!u : set us. accepts A u) ==> 
- (True#start A,True#start A) : steps (star A) (concat us)"
+ "(\<forall>u \<in> set us. accepts A u) \<Longrightarrow>
+ (True#start A,True#start A) \<in> steps (star A) (concat us)"
 apply (induct "us")
  apply (simp add:accepts_def)
 apply (simp add:accepts_def)
@@ -559,9 +559,9 @@ by(blast intro: True_True_steps_starI True_start_eps_starI in_epsclosure_steps)
 (* Better stated directly with start(star A)? Loop in star A back to start(star A)?*)
 lemma True_start_steps_star:
  "(True#start A,rr) : steps (star A) w = 
- (? us v. w = concat us @ v & 
-             (!u:set us. accepts A u) & 
-             (? r. (start A,r) : steps A v & rr = True#r))"
+ (\<exists>us v. w = concat us @ v \<and>
+             (\<forall>u\<in>set us. accepts A u) \<and>
+             (\<exists>r. (start A,r) \<in> steps A v \<and> rr = True#r))"
 apply (rule iffI)
  apply (erule True_start_steps_starD)
 apply (clarify)
@@ -571,7 +571,7 @@ done
 (** the start state **)
 
 lemma start_step_star[iff]:
-  "!!A. (start(star A),r) : step (star A) a = (a=None & r = True#start A)"
+  "\<And>A. (start(star A),r) : step (star A) a = (a=None \<and> r = True#start A)"
 by (simp add:star_def step_def)
 
 lemmas epsclosure_start_step_star =
@@ -579,7 +579,7 @@ lemmas epsclosure_start_step_star =
 
 lemma start_steps_star:
  "(start(star A),r) : steps (star A) w = 
- ((w=[] & r= start(star A)) | (True#start A,r) : steps (star A) w)"
+ ((w=[] \<and> r= start(star A)) | (True#start A,r) : steps (star A) w)"
 apply (rule iffI)
  apply (case_tac "w")
   apply (simp add: epsclosure_start_step_star)
@@ -592,16 +592,16 @@ apply (erule disjE)
 apply (blast intro: in_steps_epsclosure)
 done
 
-lemma fin_star_True[iff]: "!!A. fin (star A) (True#p) = fin A p"
+lemma fin_star_True[iff]: "\<And>A. fin (star A) (True#p) = fin A p"
 by (simp add:star_def)
 
-lemma fin_star_start[iff]: "!!A. fin (star A) (start(star A))"
+lemma fin_star_start[iff]: "\<And>A. fin (star A) (start(star A))"
 by (simp add:star_def)
 
 (* too complex! Simpler if loop back to start(star A)? *)
 lemma accepts_star:
  "accepts (star A) w = 
- (? us. (!u : set(us). accepts A u) & (w = concat us) )"
+ (\<exists>us. (\<forall>u \<in> set(us). accepts A u) \<and> (w = concat us))"
 apply(unfold accepts_def)
 apply (simp add: start_steps_star True_start_steps_star)
 apply (rule iffI)
@@ -628,7 +628,7 @@ done
 (***** Correctness of r2n *****)
 
 lemma accepts_rexp2nae:
- "!!w. accepts (rexp2nae r) w = (w : lang r)"
+ "\<And>w. accepts (rexp2nae r) w = (w : lang r)"
 apply (induct "r")
      apply (simp add: accepts_def)
     apply simp
