thys/Functional-Automata/Automata.thy
@@ -9,19 +9,19 @@ imports DA NAe
 begin
 
 definition
- na2da :: "('a,'s)na => ('a,'s set)da" where
-"na2da A = ({start A}, %a Q. Union(next A a ` Q), %Q. ? q:Q. fin A q)"
+ na2da :: "('a,'s)na \<Rightarrow> ('a,'s set)da" where
+"na2da A = ({start A}, \<lambda>a Q. Union(next A a ` Q), \<lambda>Q. \<exists>q\<in>Q. fin A q)"
 
 definition
- nae2da :: "('a,'s)nae => ('a,'s set)da" where
+ nae2da :: "('a,'s)nae \<Rightarrow> ('a,'s set)da" where
 "nae2da A = ({start A},
-              %a Q. Union(next A (Some a) ` ((eps A)^* `` Q)),
-              %Q. ? p: (eps A)^* `` Q. fin A p)"
+              \<lambda>a Q. Union(next A (Some a) ` ((eps A)\<^sup>* `` Q)),
+              \<lambda>Q. \<exists>p \<in> (eps A)\<^sup>* `` Q. fin A p)"
 
 (*** Equivalence of NA and DA ***)
 
 lemma DA_delta_is_lift_NA_delta:
- "!!Q. DA.delta (na2da A) w Q = Union(NA.delta A w ` Q)"
+ "\<And>Q. DA.delta (na2da A) w Q = Union(NA.delta A w ` Q)"
 by (induct w)(auto simp:na2da_def)
 
 lemma NA_DA_equiv:
@@ -33,7 +33,7 @@ done
 (*** Direct equivalence of NAe and DA ***)
 
 lemma espclosure_DA_delta_is_steps:
- "!!Q. (eps A)^* `` (DA.delta (nae2da A) w Q) = steps A w `` Q"
+ "\<And>Q. (eps A)\<^sup>* `` (DA.delta (nae2da A) w Q) = steps A w `` Q"
 apply (induct w)
  apply(simp)
 apply (simp add: step_def nae2da_def)
@@ -43,7 +43,7 @@ done
 lemma NAe_DA_equiv:
   "DA.accepts (nae2da A) w = NAe.accepts A w"
 proof -
-  have "!!Q. fin (nae2da A) Q = (EX q : (eps A)^* `` Q. fin A q)"
+  have "\<And>Q. fin (nae2da A) Q = (\<exists>q \<in> (eps A)\<^sup>* `` Q. fin A q)"
     by(simp add:nae2da_def)
   thus ?thesis
     apply(simp add:espclosure_DA_delta_is_steps NAe.accepts_def DA.accepts_def)
