thys/Functional-Automata/MaxChop.thy
@@ -8,22 +8,22 @@ theory MaxChop
 imports MaxPrefix
 begin
 
-type_synonym 'a chopper = "'a list => 'a list list * 'a list"
+type_synonym 'a chopper = "'a list \<Rightarrow> 'a list list * 'a list"
 
 definition
- is_maxchopper :: "('a list => bool) => 'a chopper => bool" where
+ is_maxchopper :: "('a list \<Rightarrow> bool) \<Rightarrow> 'a chopper \<Rightarrow> bool" where
 "is_maxchopper P chopper =
- (!xs zs yss.
+ (\<forall>xs zs yss.
     (chopper(xs) = (yss,zs)) =
-    (xs = concat yss @ zs & (!ys : set yss. ys ~= []) &
+    (xs = concat yss @ zs \<and> (\<forall>ys \<in> set yss. ys \<noteq> []) \<and>
      (case yss of
-        [] => is_maxpref P [] xs
-      | us#uss => is_maxpref P us xs & chopper(concat(uss)@zs) = (uss,zs))))"
+        [] \<Rightarrow> is_maxpref P [] xs
+      | us#uss \<Rightarrow> is_maxpref P us xs \<and> chopper(concat(uss)@zs) = (uss,zs))))"
 
 definition
- reducing :: "'a splitter => bool" where
+ reducing :: "'a splitter \<Rightarrow> bool" where
 "reducing splitf =
- (!xs ys zs. splitf xs = (ys,zs) & ys ~= [] --> length zs < length xs)"
+ (\<forall>xs ys zs. splitf xs = (ys,zs) \<and> ys \<noteq> [] \<longrightarrow> length zs < length xs)"
 
 function chop :: "'a splitter \<Rightarrow> 'a list \<Rightarrow> 'a list list \<times> 'a list" where
   [simp del]: "chop splitf xs = (if reducing splitf
@@ -34,13 +34,13 @@ function chop :: "'a splitter \<Rightarrow> 'a list \<Rightarrow> 'a list list \
                       else undefined)"
 by pat_completeness auto
 
-termination apply (relation "measure (length o snd)")
+termination apply (relation "measure (length \<circ> snd)")
 apply (auto simp: reducing_def)
 apply (case_tac "splitf xs")
 apply auto
 done
 
-lemma chop_rule: "reducing splitf ==>
+lemma chop_rule: "reducing splitf \<Longrightarrow>
   chop splitf xs = (let (pre, post) = splitf xs
                     in if pre = [] then ([], xs)
                        else let (xss, zs) = chop splitf post
@@ -49,23 +49,23 @@ apply (simp add: chop.simps)
 apply (simp add: Let_def split: prod.split)
 done
 
-lemma reducing_maxsplit: "reducing(%qs. maxsplit P ([],qs) [] qs)"
+lemma reducing_maxsplit: "reducing(\<lambda>qs. maxsplit P ([],qs) [] qs)"
 by (simp add: reducing_def maxsplit_eq)
 
 lemma is_maxsplitter_reducing:
- "is_maxsplitter P splitf ==> reducing splitf"
+ "is_maxsplitter P splitf \<Longrightarrow> reducing splitf"
 by(simp add:is_maxsplitter_def reducing_def)
 
-lemma chop_concat[rule_format]: "is_maxsplitter P splitf ==>
-  (!yss zs. chop splitf xs = (yss,zs) --> xs = concat yss @ zs)"
+lemma chop_concat[rule_format]: "is_maxsplitter P splitf \<Longrightarrow>
+  (\<forall>yss zs. chop splitf xs = (yss,zs) \<longrightarrow> xs = concat yss @ zs)"
 apply (induct xs rule:length_induct)
 apply (simp (no_asm_simp) split del: if_split
             add: chop_rule[OF is_maxsplitter_reducing])
 apply (simp add: Let_def is_maxsplitter_def split: prod.split)
 done
 
-lemma chop_nonempty: "is_maxsplitter P splitf ==>
-  !yss zs. chop splitf xs = (yss,zs) --> (!ys : set yss. ys ~= [])"
+lemma chop_nonempty: "is_maxsplitter P splitf \<Longrightarrow>
+  \<forall>yss zs. chop splitf xs = (yss,zs) \<longrightarrow> (\<forall>ys \<in> set yss. ys \<noteq> [])"
 apply (induct xs rule:length_induct)
 apply (simp (no_asm_simp) add: chop_rule is_maxsplitter_reducing)
 apply (simp add: Let_def is_maxsplitter_def split: prod.split)
